
\(\therefore \sin^2 a + 4\sin \alpha \cos \alpha +4\cos^2 \alpha = \frac{5}{2}\) ,  

\(\therefore \tan^2 a + 4\tan \alpha +4 = \frac{5}{2}\) , 解得 \(\tan \alpha = -\frac{1}{3}\) 或 \(\tan \alpha = 3\) ,  

当 \(\tan \alpha = -\frac{1}{3}\) 时, \(\tan 2\alpha = \frac{2\times\left(-\frac{1}{3}\right)}{1 - \frac{1}{3}} = -\frac{3}{4}\) ,  

当 \(\tan \alpha = 3\) 时, \(\tan 2\alpha = \frac{1}{6} = -\frac{3}{4}\) , \(\therefore \tan 2\alpha = -\frac{3}{4}\) , 故选 B.  

8. 选 D \(\cos \left(\frac{\pi}{3} +2a\right) = -\cos \left(\frac{2\pi}{3} -2a\right) = -1 + 2\sin^2 \left(\frac{\pi}{3} -a\right) =\) \(-1 + \frac{2}{3} = -\frac{7}{6}\) , 故选 D.  

9. 选 C \(4\cos 50^{\circ} - \tan 40^{\circ}\)  

\(= 4\cos 50^{\circ} - \frac{\sin 40^{\circ}}{\cos 40^{\circ}}\)  

\(= \frac{4\sin 40^{\circ}\cos 40^{\circ} - \sin 40^{\circ}}{\cos 40^{\circ}}\)  

\(= \frac{2\sin 80^{\circ} - \sin 40^{\circ}}{\cos 40^{\circ}}\)  

\(= \frac{2\sin(50^{\circ} + 30^{\circ}) - \cos 50^{\circ}}{\cos 40^{\circ}}\)  

\(= \frac{\sqrt{3}\sin 50^{\circ}}{\cos 40^{\circ}}\)  

\(= \sqrt{3}\) , 故选 C.  

\(= \sqrt{3}\) , 故选 C.  

10. 选 A 原式 \(= \frac{\sin\frac{\pi}{9}\cos\frac{\pi}{9}\cos\frac{2\pi}{9}\cos\frac{5\pi}{9}}{\sin\frac{\pi}{9}}\)  

10. 选 A 原式 \(= \frac{\sin\frac{\pi}{9}\cos\frac{\pi}{9}\cos\frac{2\pi}{9}\cos\frac{5\pi}{9}}{\sin\frac{\pi}{9}}\)  

\(= \frac{1}{2}\sin \frac{2\pi}{9}\cos \frac{2\pi}{9}\left(-\cos \frac{4\pi}{9}\right)\)  

\(= \frac{1}{2}\sin \frac{2\pi}{9}\cos \frac{2\pi}{9}\left(-\cos \frac{4\pi}{9}\right)\)  

\(= \frac{1}{2}\sin \frac{2\pi}{9}\cos \frac{2\pi}{9}\left(-\cos \frac{4\pi}{9}\right)\)  

\(= \frac{1}{2}\sin \frac{2\pi}{9}\cos \frac{2\pi}{9}\left(-\cos \frac{4\pi}{9}\right)\)  

\(= \frac{1}{2}\sin \frac{2\pi}{9}\cos \frac{2\pi}{9}\left(-\cos \frac{4\pi}{9}\right)\)  

\(= \frac{1}{2}\sin \frac{2\pi}{9}\cos \frac{2\pi}{9}\left(-\cos \frac{4\pi}{9}\right)\)  

\(= \frac{1}{2}\sin \frac{2\pi}{9}\cos \frac{2\pi}{9}\left(-\cos \frac{4\pi}{9}\right)\)  

\(= \frac{1}{2}\sin \frac{2\pi}{9}\cos \frac{2\pi}{9}\left(-\cos \frac{4\pi}{9}\right)\)  

\(= \frac{1}{2}\sin \frac{2\pi}{9}\cos \frac{2\pi}{9}\left(-\cos \frac{4\pi}{9}\right)\)  

\(= \frac{1}{2}\sin \frac{2\pi}{9}\cos \frac{2\pi}{9}\left(-\cos \frac{4\pi}{9}\right)\)  

\(= \frac{1}{2}\sin \frac{2\pi}{9}\cos \frac{2\pi}{9}\left(-\cos \frac{4\pi}{9}\right)\)  

\(= \frac{1}{2}\sin \frac{2\pi}{9}\cos \frac{2\pi}{9}\left(-\cos \frac{4\pi}{9}\right)\)  

\(= \frac{1}{2}\sin \frac{2\pi}{9}\cos \frac{2\pi}{9}\left(-\cos \frac{4\pi}{9}\right)\)  

\(= \frac{1}{2}\sin \frac{2\pi}{9}\cos \frac{2\pi}{9}\left(-\cos \frac{4\pi}{9}\right)\)  

\(= \frac{1}{2}\sin \frac{2\pi}{9}\cos \frac{2\pi}{9}\left(-\cos \frac{4\pi}{9}\right)\)  

\(= \frac{1}{2}\sin \frac{2\pi}{9}\cos \frac{2\pi}{9}\left(-\cos \frac{4\pi}{9}\right)\)  

\(= \frac{1}{2}\sin \frac{2\pi}{9}\cos \frac{2\pi}{9}\left(-\cos \frac{4\pi}{9}\right)\)  

\(= \frac{1}{2}\sin \frac{2\pi}{9}\cos \frac{2\pi}{9}\left(-\cos \frac{4\pi}{9}\right)\)  

\(= \frac{1}{2}\sin \frac{2\pi}{9}\cos \frac{2\pi}{9}\left(-\cos \frac{4\pi}{9}\right)\)  

\(= \frac{1}{2}\sin \frac{2\pi}{9}\cos \frac{2\pi}{9}\left(-\cos \frac{4\pi}{9}\right)\)  

\(= \frac{1}{2}\sin \frac{2\pi}{9}\cos \frac{2\pi}{9}\left(-\cos \frac{4\pi}{9}\right)\)  

\(= \frac{1}{2}\sin \frac{2\pi}{9}\cos \frac{2\pi}{9}\left(-\cos \frac{4\pi}{9}\right)\)  

\(= \frac{1}{2}\sin \frac{2\pi}{9}\cos \frac{2\pi}{9}\left(-\cos \frac{4\pi}{9}\right)\)  

\(= \frac{1}{2}\sin \frac{2\pi}{9}\cos \frac{2\pi}{9}\left(-\cos \frac{4\pi}{9}\right)\)  

\(= \frac{1}{2}\sin \frac{2\pi}{9}\cos \frac{2\pi}{9}\left(-\cos \frac{4\pi}{9}\right)\)  

\(= \frac{1}{2}\sin \frac{2\pi}{9}\cos \frac{2\pi}{9}\left(-\cos \frac{4\pi}{9}\right)\)  

\(= \frac{1}{2}\sin \frac{2\pi}{9}\cos \frac{2\pi}{9}\left(-\cos \frac{4\pi}{9}\right)\)  

\(= \frac{1}{2}\sin \frac{2\pi}{9}\cos \frac{2\pi}{9}\left(-\cos \frac{4\pi}{9}\right)\)  

\(= \frac{1}{2}\sin \frac{2\pi}{9}\cos \frac{2\pi}{9}\left(-\cos \frac{4\pi}{9}\right)\)  

\(= \frac{1}{2}\sin \frac{2\pi}{9}\cos \frac{2\pi}{9}\left(-\cos \frac{4\pi}{9}\right)\)  

\(= \frac{1}{2}\sin \frac{2\pi}{9}\cos \frac{2\pi}{9}\left(-\cos \frac{4\pi}{9}\right)\)  

\(= \frac{1}{2}\sin \frac{2\pi}{9}\cos \frac{2\pi}{9}\left(-\cos \frac{4\pi}{9}\right)\)  

\(= \frac{1}{2}\sin \frac{2\pi}{9}\cos \frac{2\pi}{9}\left(-\cos \frac{4\pi}{9}\right)\)  

\(= \frac{1}{2}\sin \frac{2\pi}{9}\cos \frac{2\pi}{9}\left(-\cos \frac{4\pi}{9}\right)\)  

\(= \frac{1}{2}\sin \frac{2\pi}{9}\cos \frac{2\pi}{9}\left(-\cos \frac{4\pi}{9}\right)\)  

\(= \frac{1}{2}\sin \frac{2\pi}{9}\cos \frac{2\pi}{9}\left(-\cos \frac{4\pi}{9}\right)\)  

\(= \frac{1}{2}\sin \frac{2\pi}{9}\cos \frac{2\pi}{9}\left(-\cos \frac{4\pi}{9}\right)\)  

\(= \frac{1}{2}\sin \frac{2\pi}{9}\cos \frac{2\pi}{9}\left(-\cos \frac{4\pi}{9}\right)\)  

\(= \frac{1}{2}\sin \frac{2\pi}{9}\cos \frac{2\pi}{9}\left(-\cos \frac{4\pi}{9}\right)\)  

\(= \frac{1}{2}\sin \frac{2\pi}{9}\cos \frac{2\pi}{9}\left(-\cos \frac{4\pi}{9}\right)\)  

\(= \frac{1}{2}\sin \frac{2\pi}{9}\cos \frac{2\pi}{9}\left(-\cos \frac{4\pi}{9}\right)\)  

\(= \frac{1}{2}\sin \frac{2\pi}{9}\cos \frac{2\pi}{9}\left(-\cos \frac{4\pi}{9}\right)\)  

\(= \frac{1}{2}\sin \frac{2\pi}{9}\cos \frac{2\pi}{9}\left(-\cos \frac{4\pi}{9}\right)\)  

\(= \frac{1}{2}\sin \frac{2\pi}{9}\cos \frac{2\pi}{9}\left(-\cos \frac{4\pi}{9}\right)\)  

\(= \frac{1}{2}\sin \frac{2\pi}{9}\cos \frac{2\pi}{9}\left(-\cos \frac{4\pi}{9}\right)\)  

\(= \frac{1}{2}\sin \frac{2\pi}{9}\cos \frac{2\pi}{9}\left(-\cos \frac{4\pi}{9}\right)\)  

\(= \frac{1}{2}\sin \frac{2\pi}{9}\cos \frac{2\pi}{9}\left(-\cos \frac{4\pi}{9}\right)\)  

\(= \frac{1}{2}\sin \frac{2\pi}{9}\cos \frac{2\pi}{9}\left(-\cos \frac{4\pi}{9}\right)\)  

\(= \frac{1}{2}\sin \frac{2\pi}{9}\cos \frac{2\pi}{9}\left(-\cos \frac{4\pi}{9}\right)\)  

\(= \frac{1}{2}\sin \frac{2\pi}{9}\cos \frac{2\pi}{9}\left(-\cos \frac{4\pi}{9}\right)\)  

\(= \frac{1}{2}\sin \frac{2\pi}{9}\cos \frac{2\pi}{9}\left(-\cos \frac{4\pi}{9}\right)\)  

\(= \frac{1}{2}\sin \frac{2\pi}{9}\cos \frac{2\pi}{9}\left(-\cos \frac{4\pi}{9}\right)\)  

\(= \frac{1}{2}\sin \frac{2\pi}{9}\cos \frac{2\pi}{9}\left(-\cos \frac{4\pi}{9}\right)\)  

\(= \frac{1}{2}\sin \frac{2\pi}{9}\cos \frac{2\pi}{9}\left(-\cos \frac{4\pi}{9}\right)\)  

\(= \frac{1}{2}\sin \frac{2\pi}{9}\cos \frac{2\pi}{9}\left(-\cos \frac{4\pi}{9}\right)\)  

\(= \frac{1}{2}\sin \frac{2\pi}{9}\cos \frac{2\pi}{9}\left(-\cos \frac{4\pi}{9}\right)\)  

\(= \frac{1}{2}\sin \frac{2\pi}{9}\cos \frac{2\pi}{9}\left(-\cos \frac{4\pi}{9}\right)\)  

\(= \frac{1}{2}\sin \frac{2\pi}{9}\cos \frac{2\pi}{9}\left(-\cos \frac{4\pi}{9}\right)\)  

\(= \frac{1}{2}\sin \frac{2\pi}{9}\cos \frac{2\pi}{9}\left(-\cos \frac{4\pi}{9}\right)\)  

\(= \frac{1}{2}\sin \frac{2\pi}{9}\cos \frac{2\pi}{9}\left(-\cos \frac{4\pi}{9}\right)\)  

\(= \frac{1}{2}\sin \frac{2\pi}{9}\cos \frac{2\pi}{9}\left(-\cos \frac{4\pi}{9}\right)\)  

\(= \frac{1}{2}\sin \frac{2\pi}{9}\cos \frac{2\pi}{9}\left(-\cos \frac{4\pi}{9}\right)\)  

\(= \frac{1}{2}\sin \frac{2\pi}{9}\cos \frac{2\pi}{9}\left(-\cos \frac{4\pi}{9}\right)\)  

\(= \frac{1}{2}\sin \frac{2\pi}{9}\cos \frac{2\pi}{9}\left(-\cos \frac{4\pi}{9}\right)\)  

\(= \frac{1}{2}\sin \frac{2\pi}{9}\cos \frac{2\pi}{9}\left(-\cos \frac{4\pi}{9}\right)\)  

\(= \frac{1}{2}\sin \frac{2\pi}{9}\cos \frac{2\pi}{9}\left(-\cos \frac{4\pi}{9}\right)\)  

\(= \frac{1}{2}\sin \frac{2\pi}{9}\cos \frac{2\pi}{9}\left(-\cos \frac{4\pi}{9}\right)\)  

\(= \frac{1}{2}\sin \frac{2\pi}{9}\cos \frac{2\pi}{9}\left(-\cos \frac{4\pi}{9}\right)\)  

\(= \frac{1}{2}\sin \frac{2\pi}{9}\cos \frac{2\pi}{9}\left(-\cos \frac{4\pi}{9}\right)\)  

\(= \frac{1}{2}\sin \frac{2\pi}{9}\cos \frac{2\pi}{9}\left(-\cos \frac{4\pi}{9}\right)\)  

\(= \frac{1}{2}\sin \frac{2\pi}{9}\cos \frac{2\pi}{9}\left(-\cos \frac{4\pi}{9}\right)\)  

\(= \frac{1}{2}\sin \frac{2\pi}{9}\cos \frac{2\pi}{9}\left(-\cos \frac{4\pi}{9}\right)\)  

\(= \frac{1}{2}\sin \frac{2\pi}{9}\cos \frac{2\pi}{9}\left(-\cos \frac{4\pi}{9}\right)\)  

\(= \frac{1}{2}\sin \frac{2\pi}{9}\cos \frac{2\pi}{9}\left(-\cos \frac{4\pi}{9}\right)\)  

\(= \frac{1}{2}\sin \frac{2\pi}{9}\cos \frac{2\pi}{9}\left(-\cos \frac{4\pi}{9}\right)\)  

\(= \frac{1}{2}\sin \frac{2\pi}{9}\cos \frac{2\pi}{9}\left(-\cos \frac{4\pi}{9}\right)\)  

\(= \frac{1}{2}\sin \frac{2\pi}{9}\cos \frac{2\pi}{9}\left(-\cos \frac{4\pi}{9}\right)\)  

\(= \frac{1}{2}\sin \frac{2\pi}{9}\cos \frac{2\pi}{9}\left(-\cos \frac{4\pi}{9}\right)\)  

\(= \frac{1}{2}\sin \frac{2\pi}{9}\cos \frac{2\pi}{9}\left(-\cos \frac{4\pi}{9}\right)\)  

\(= \frac{1}{2}\sin \frac{2\pi}{9}\cos \frac{2\pi}{9}\left(-\cos \frac{4\pi}{9}\right)\)  

\(= \frac{1}{2}\sin \frac{2\pi}{9}\cos \frac{2\pi}{9}\left(-\cos \frac{4\pi}{9}\right)\)  

\(= \frac{1}{2}\sin \frac{2\pi}{9}\cos \frac{2\pi}{9}\left(-\cos \frac{4\pi}{9}\right)\)  

\(= \frac{1}{2}\sin \frac{2\pi}{9}\cos \frac{2\pi}{9}\left(-\cos \frac{4\pi}{9}\right)\)  

\(= \frac{1}{2}\sin \frac{2\pi}{9}\cos \frac{2\pi}{9}\left(-\cos \frac{4\pi}{9}\right)\)  

\(= \frac{1}{2}\sin \frac{2\pi}{9}\cos \frac{2\pi}{9}\left(-\cos \frac{4\pi}{9}\right)\)  

\(= \frac{1}{2}\sin \frac{2\pi}{9}\cos \frac{2\pi}{9}\left(-\cos \frac{4\pi}{9}\right)\)  

\(= \frac{1}{2}\sin \frac{2\pi}{9}\cos \frac{2\pi}{9}\left(-\cos \frac{4\pi}{9}\right)\)  

\(= \frac{1}{2}\sin \frac{2\pi}{9}\cos \frac{2\pi}{9}\left(-\cos \frac{4\pi}{9}\right)\)  

\(= \frac{1}{2}\sin \frac{2\pi}{9}\cos \frac{2\pi}{9}\left(-\cos \frac{4\pi}{9}\right)\)  

\(= \frac{1}{2}\sin \frac{2\pi}{9}\cos \frac{2\pi}{9}\left(-\cos \frac{4\pi}{9}\right)\)  

\(= \frac{1}{2}\sin \frac{2\pi}{9}\cos \frac{2\pi}{9}\left(-\cos \frac{4\pi}{9}\right)\)  

\(= \frac{1}{2}\sin \frac{2\pi}{9}\cos \frac{2\pi}{9}\left(-\cos \frac{4\pi}{9}\right)\)  

\(= \frac{1}{2}\sin \frac{2\pi}{9}\cos \frac{2\pi}{9}\left(-\cos \frac{4\pi}{9}\right)\)  

\(= \frac{1}{2}\sin \frac{2\pi}{9}\cos \frac{2\pi}{9}\left(-\cos \frac{4\pi}{9}\right)\)  

\(= \frac{1}{2}\sin \frac{2\pi}{9}\cos \frac{2\pi}{9}\left(-\cos \frac{4\pi}{9}\right)\)  

\(= \frac{1}{2}\sin \frac{2\pi}{9}\cos \frac{2\pi}{9}\left(-\cos \frac{4\pi}{9}\right)\)  

\(= \frac{1}{2}\sin \frac{2\pi}{9}\cos \frac{2\pi}{9}\left(-\cos \frac{4\pi}{9}\right)\)  

\(= \frac{1}{2}\sin \frac{2\pi}{9}\cos \frac{2\pi}{9}\left(-\cos \frac{4\pi}{9}\right)\)  

\(= \frac{1}{2}\sin \frac{2\pi}{9}\cos \frac{2\pi}{9}\left(-\cos \frac{4\pi}{9}\right)\)  

\(= \frac{1}{2}\sin \frac{2\pi}{9}\cos \frac{2\pi}{9}\left(-\cos \frac{4\pi}{9}\right)\)  

\(= \frac{1}{2}\sin \frac{2\pi}{9}\cos \frac{2\pi}{9}\left(-\cos \frac{4\pi}{9}\right)\)  

\(= \frac{1}{2}\sin \frac{2\pi}{9}\cos \frac{2\pi}{9}\left(-\cos \frac{4\pi}{9}\right)\)  

\(= \frac{1}{2}\sin \frac{2\pi}{9}\cos \frac{2\pi}{9}\left(-\cos \frac{4\pi}{9}\right)\)  

\(= \frac{1}{2}\sin \frac{2\pi}{9}\cos \frac{2\pi}{9}\left(-\cos \frac{4\pi}{9}\right)\)  

\(= \frac{1}{2}\sin \frac{2\pi}{9}\cos \frac{2\pi}{9}\left(-\cos \frac{4\pi}{9}\right)\)  

\(= \frac{1}{2}\sin \frac{2\pi}{9}\cos \frac{2\pi}{9}\left(-\cos \frac{4\pi}{9}\right)\)  

\(= \frac{1}{2}\sin \frac{2\pi}{9}\cos \frac{2\pi}{9}\left(-\cos \frac{4\pi}{9}\right)\)  

\(= \frac{1}{2}\sin \frac{2\pi}{9}\cos \frac{2\pi}{9}\left(-\cos \frac{4\pi}{9}\right)\)  

\(= \frac{1}{2}\sin \frac{2\pi}{9}\cos \frac{2\pi}{9}\left(-\cos \frac{4\pi}{9}\right)\)  

<|ref|>text<|/ref|><|det|>[[70, 985, 131, 