Proof Firstly, from (9.14) we get

\[
\left| P_n - \sum_{k=1}^n \frac{\mu(k)}{k^2} \right| = \left| \sum_{k=1}^n \mu(k) \left( \frac{1}{n^2} \left\lfloor \frac{n}{k} \right\rfloor^2 - \frac{1}{k^2} \right) \right|
\]
\[
\leq \sum_{k=1}^n \left| \frac{1}{k^2} - \frac{1}{n^2} \left\lfloor \frac{n}{k} \right\rfloor^2 \right|.
\] (9.15)

In order to estimate the last sum above, we claim that, given natural numbers \( n \) and \( k \) such that \( 1 \leq k \leq n \), we have

\[
\left| \frac{1}{k^2} - \frac{1}{n^2} \left\lfloor \frac{n}{k} \right\rfloor^2 \right| < \frac{2}{nk} - \frac{1}{n^2}.
\]

Indeed,

\[
\frac{n}{k} - 1 < \left\lfloor \frac{n}{k} \right\rfloor \leq \frac{n}{k} \implies \frac{n^2}{k^2} - \frac{2n}{k} + 1 < \left\lfloor \frac{n}{k} \right\rfloor^2 \leq \frac{n^2}{k^2}
\]
\[
\implies \frac{1}{k^2} - \frac{2}{kn} + \frac{1}{n^2} < \frac{1}{n^2} \left\lfloor \frac{n}{k} \right\rfloor^2 \leq \frac{1}{k^2}
\]
\[
\implies 0 \leq \frac{1}{k^2} - \frac{1}{n^2} \left\lfloor \frac{n}{k} \right\rfloor^2 < \frac{2}{kn} - \frac{1}{n^2},
\]

as wished.

Back to (9.15), we obtain from the above estimates that

\[
\left| P_n - \sum_{k=1}^n \frac{\mu(k)}{k^2} \right| < \sum_{k=1}^n \left( \frac{2}{nk} - \frac{1}{n^2} \right) = \frac{2}{n} \sum_{k=1}^n \frac{1}{k} - \frac{1}{n}.
\]

Now, from L'HÃ´pital's rule we get

\[
\frac{2}{n} \sum_{k=1}^n \frac{1}{k} < \frac{2}{n} \left( 1 + \int_1^n \frac{1}{t} dt \right) = \frac{2}{n} (\log n + 1) \to 0
\]

as \( n \to +\infty \). Hence,

\[
\lim_{n \to +\infty} \left( \frac{2}{n} \sum_{k=1}^n \frac{1}{k} - \frac{1}{n} \right) = 0,
\]

and our previous estimates assure that