the form \( frf^{-1}r^{-1} \) for \( f \in F \) and \( r \in R \). These results led S. Eilenberg, S. Mac Lane, Hopf, H. Freudenthal, and B. Eckmann to create cohomology of groups.

In what follows, we will write \( \mathrm{Hom}_G \) instead of \( \mathrm{Hom}_{\mathbb{Z}G} \) and \( \otimes_G \) instead of \( \otimes_{\mathbb{Z}G} \). Because of the special role of the trivial \( G \)-module \( \mathbb{Z} \), the augmentation

\[
\varepsilon : \mathbb{Z}G \to \mathbb{Z},
\]

defined by

\[
\varepsilon : \sum_{x \in G} m_x x \mapsto \sum_{x \in G} m_x,
\]

is important. Recall that we have seen, in Exercise 8.37 on page 573, that \( \varepsilon \) is a surjective ring homomorphism, and so its kernel, \( \mathcal{G} \), is a two-sided ideal in \( \mathbb{Z}G \), called the **augmentation ideal**. Thus, there is an exact sequence

\[
0 \to \mathcal{G} \to \mathbb{Z}G \xrightarrow{\varepsilon} \mathbb{Z} \to 0.
\]

**Proposition 10.103.** *Let \( G \) be a group with augmentation ideal \( \mathcal{G} \). As an abelian group, \( \mathcal{G} \) is free abelian with basis \( G - 1 = \{ x - 1 : x \in G, x \neq 1 \} \).*

*Proof.* An element \( u = \sum_x m_x x \in \mathbb{Z}G \) lies in \( \ker \varepsilon = \mathcal{G} \) if and only if \( \sum_x m_x = 0 \). Therefore, if \( u \in \mathcal{G} \), then

\[
u = u - (\sum_x m_x) 1 = \sum_x m_x (x - 1).
\]

Thus, \( \mathcal{G} \) is generated by the nonzero \( x - 1 \) for \( x \in G \).

Suppose that \( \sum_{x \neq 1} n_x (x - 1) = 0 \). Then \( \sum_{x \neq 1} n_x x - (\sum_{x \neq 1} n_x) 1 = 0 \) in \( \mathbb{Z}G \), which, as an abelian group, is free abelian with basis the elements of \( G \). Hence, \( n_x = 0 \) for all \( x \neq 1 \). Therefore, the nonzero \( x - 1 \) comprise a basis of \( \mathcal{G} \). \( \bullet \)

We begin by examining homology groups.

**Proposition 10.104.** *If \( A \) is a \( G \)-module, then*

\[
H_0(G, A) = \mathbb{Z} \otimes_G A \cong A / \mathcal{G}A.
\]

*Proof.* By definition, \( H_0(G, A) = \mathrm{Tor}_0^{\mathbb{Z}G}(\mathbb{Z}, A) = \mathbb{Z} \otimes_G A \). Applying the right exact functor \( \otimes_G A \) to the exact sequence

\[
0 \to \mathcal{G} \to \mathbb{Z}G \to \mathbb{Z} \to 0
\]

gives exactness of the first row of the following commutative diagram:

\[
\begin{array}{ccccccccc}
\mathcal{G} \otimes_G A & \longrightarrow & \mathbb{Z}G \otimes_G A & \longrightarrow & \mathbb{Z} \otimes_G A & \longrightarrow & 0 \\
\downarrow & & \downarrow & & \downarrow & & \\
\mathcal{G}A & \longrightarrow & A & \longrightarrow & A / \mathcal{G}A & \longrightarrow & 0
\end{array}
\]

The two solid vertical arrows are given by \( u \otimes a \mapsto ua \). By Proposition 8.93, there is an isomorphism \( \mathbb{Z} \otimes_G A \cong A / \mathcal{G}A \). \( \bullet \)