The Quotient Rule

We find a rule for differentiating the quotient of two differentiable functions \( u = f(x) \) and \( v = g(x) \) in much the same way that we found the Product Rule.

If \( x, u, \) and \( v \) change by amounts \( \Delta x, \Delta u, \) and \( \Delta v, \) then the corresponding change in the quotient \( u/v \) is

\[
\Delta \left( \frac{u}{v} \right) = \frac{u + \Delta u}{v + \Delta v} - \frac{u}{v} = \frac{(u + \Delta u)v - u(v + \Delta v)}{v(v + \Delta v)}
\]

\[
= \frac{v \Delta u - u \Delta v}{v(v + \Delta v)}
\]