\[
x_1 \quad -2x_2 \quad +x_3 \quad = 0 \\
2x_2 \quad -8x_3 \quad = 8 \\
-3x_2 \quad +13x_3 \quad = -9
\]

\[
\begin{bmatrix}
1 & -2 & 1 & 0 \\
0 & 2 & -8 & 8 \\
0 & -3 & 13 & -9
\end{bmatrix}
\]

Changing the coefficient of \( x_2 \) from 2 to 1.
• The purpose of this step is to simplify the calculation in the next steps.
• To do it, we multiply the 2nd equation by \( \frac{1}{2} \).

\[
x_1 \quad -2x_2 \quad +x_3 \quad = 0 \\
x_2 \quad -4x_3 \quad = 4 \\
-3x_2 \quad +13x_3 \quad = -9
\]

\[
\begin{bmatrix}
1 & -2 & 1 & 0 \\
0 & 1 & -4 & 4 \\
0 & -3 & 13 & -9
\end{bmatrix}
\]