<|ref|>text<|/ref|><|det|>[[100, 75, 636, 96]]<|/det|>
(II)解法1:由(I)知, \(\angle A^{\prime}O C = 120^{\circ} - - - - - - - - - - - - - - - - - - - - - - - - - - - - - - - - - - - - - - - -\) 6分  

<|ref|>text<|/ref|><|det|>[[140, 100, 912, 150]]<|/det|>
如图建系 \(O - x y z\) , \(B(1,0,0)\) ,设 \(O C = b,O A^{\prime} = a\) ,则 \(C(0,b,0)\) , \(A^{\prime}(0, - \frac{1}{2} a,\frac{\sqrt{3}}{2} a)\) \(\overrightarrow{B C} = (- 1,b,0) - - - - - - - - - - - - - - - - - - - - - - - - - - - - - - - - - - - - - - - -\) 8分  

<|ref|>text<|/ref|><|det|>[[142, 166, 620, 187]]<|/det|>
平面 \(A^{\prime}D B\) 的法向量为 \(\vec{n} = \left(0,\sqrt{3},1\right)\) - - - - - - - - - - - - - - - - - - - - - - - - - - - - - - - - - - - - - - - - 10分  

<|ref|>text<|/ref|><|det|>[[142, 195, 568, 250]]<|/det|>
\(\sin 45^{\circ} = \left|\cos \left\langle \vec{n},B C\right\rangle \right| = \left|\frac{\vec{n}\cdot B C}{\left|\vec{n}\right|\left|B C\right|}\right|\) - - - - - - - - - - - - - - - - - - - - - - - - - - - - - - - - - - - - - - - - 11分  

<|ref|>text<|/ref|><|det|>[[142, 255, 520, 275]]<|/det|>
解得 \(b = \sqrt{2}\) , \(B C = \sqrt{3}\) - - - - - - - - - - - - - - - - - - - - - - - - - - - - - - - - - - - - - - - - 12分  

<|ref|>text<|/ref|><|det|>[[142, 277, 600, 296]]<|/det|>
解法2:由(I)知, \(\angle A^{\prime}O C = 120^{\circ} - - - - - - - - - - - - - - - - - - - - - - - - - - - - - - - - - - - - - - - - 6\) 分  

<|ref|>text<|/ref|><|det|>[[142, 297, 490, 315]]<|/det|>
过 \(c\) 作 \(C H\perp A^{\prime}O\) , \(B D\perp\) 平面 \(A^{\prime}O C\) ,  

<|ref|>text<|/ref|><|det|>[[142, 316, 530, 333]]<|/det|>
\(\therefore B D\perp C H\) , \(C H\perp A^{\prime}O\) , \(C H\perp\) 平面 \(A^{\prime}B D\)  

<|ref|>text<|/ref|><|det|>[[142, 335, 595, 353]]<|/det|>
\(\angle C B H\) 就是 \(B C\) 与平面 \(\Delta A^{\prime}B D\) 所成角- - - - - - - - - - - - - - - - - - - - - - - - - - - - - - - - - - - - - - - - - 9分  

<|ref|>text<|/ref|><|det|>[[142, 355, 565, 390]]<|/det|>
设 \(C O = x\) ,则 \(C H = \frac{\sqrt{3}}{2} x\) , \(C B = \sqrt{2} C H = \frac{\sqrt{6}}{2} x\)  

<|ref|>equation<|/ref|><|det|>[[142, 394, 560, 432]]<|/det|>
\[C B = \sqrt{O B^{2} + O C^{2}} = \sqrt{1 + x^{2}}~,~\mathbb{H}\mathbb{H}\frac{\sqrt{6}}{2} x = \sqrt{1 + x^{2}}\]  

<|ref|>text<|/ref|><|det|>[[142, 435, 506, 456]]<|/det|>
解得 \(x = \sqrt{2}\) , \(B C = \sqrt{3}\) - - - - - - - - - - - - - - - - - - - - - - - - - - - - - - - - - - - - - - - - 12分  

<|ref|>text<|/ref|><|det|>[[61, 459, 133, 476]]<|/det|>
21. 解:  

<|ref|>text<|/ref|><|det|>[[100, 480, 790, 604]]<|/det|>
(I)联立方程组 \(\left\{ \begin{array}{l l}{y = k x + 1}\\ {x^{2} - 4y^{2} = 4} \end{array} \right.\) 消 \(y\) 得: \(\left(1 - 4k^{2}\right)x^{2} - 8k x - 8 = 0\) - - - - - - - - - - - - - - - - - - - - - - - - - - - - - - - - - - - - - - - - 2分 \(\left\{ \begin{array}{l l}{1 - 4k^{2}\neq 0}\\ {\Delta = 32 - 64k^{2} > 0} \end{array} \right.\) 解得 \(- \frac{\sqrt{2}}{2} < k< \frac{\sqrt{2}}{2}\) 且 \(k\neq \pm \frac{1}{2}\) - - - - - - - - - - - - - - - - - - - - - - - - - - - - - - - - - - - - - - - - 5分  

<|ref|>text<|/ref|><|det|>[[100, 612, 671, 633]]<|/det|>
(II)设 \(M\) , \(N\) 坐标分别为 \(\left(x_{1},y_{1}\right),\left(x_{2},y_{2}\right)\) , \(A\left(- 2,0\right)\) ,由(I)知  

<|ref|>text<|/ref|><|det|>[[140, 638, 470, 720]]<|/det|>
\(\left\{ \begin{array}{l l}{x_{1} + x_{2} = \frac{8k}{1 - 4k^{2}}}\\ {x_{1}\cdot x_{2} = \frac{- 8}{1 - 4k^{2}}} \end{array} \right.\) - - - - - - - - - - - - - - - - - - - - - - - - - - - - - - - - - - - - - - - - 6分  

<|ref|>text<|/ref|><|det|>[[140, 726, 770, 770]]<|/det|>
直线 \(M A\) 的方程为 \(y = \frac{y_{1}}{x_{1} + 2}\left(x + 2\right)\) ,令 \(x = 0\) 可得点 \(P\) 坐标为 \(\left(0,\frac{2y_{1}}{x_{1} + 2}\right)\)  

<|ref|>text<|/ref|><|det|>[[142, 774, 620, 812]]<|/det|>
同理点 \(Q\) 坐标为 \(\left(0,\frac{2y_{2}}{x_{2} + 2}\right)\) - - - - - - - - - - - - - - - - - - - - - - - - - - - - - - - - - - - - - - - - 8分  

<|ref|>equation<|/ref|><|det|>[[142, 815, 606, 860]]<|/det|>
\[|P Q| = 1\Rightarrow \left|\frac{y_{1}}{x_{1} + 2} -\frac{y_{2}}{x_{2} + 2}\right| = \frac{1}{2}\Rightarrow \left|\frac{\left(x_{1} - x_{2}\right)\left(1 - 2k\right)}{\left(x_{1} + 2\right)\left(x_{2} + 2\right)}\right| = \frac{1}{2}\]  

<|ref|>equation<|/ref|><|det|>[[142, 864, 606, 894]]<|/det|>
\[4\sqrt{2}\sqrt{1 - 2k^{2}}\left(1 - 2k\right) = 2\left(2k - 1\right)^{2} - \dots \dots \dots \dots \dots \dots \dots \dots \dots \dots \dots \dots \dots \dots \dots \dots \dots \dots \dots \dots \quad (10分)\]