<|ref|>text<|/ref|><|det|>[[68, 100, 275, 121]]<|/det|>
19. 解：（1）取 \(EF\) 的中点 \(G\) ，连接 \(DG\) ， \(CG\)  

<|ref|>text<|/ref|><|det|>[[68, 128, 370, 151]]<|/det|>
四边形 \(ADE_{1}F_{1}\) 和 \(BCE_{2}F_{2}\) 都是菱形， \(\angle DE_{1}F_{1} = \angle CE_{2}F_{2} = 60^{\circ}\)  

<|ref|>text<|/ref|><|det|>[[68, 161, 300, 204]]<|/det|>
\(\therefore DG\bot EF\) 又 \(BC = 2\)  

<|ref|>text<|/ref|><|det|>[[68, 214, 333, 240]]<|/det|>
\(\therefore DG = CG = \sqrt{3}\)  

<|ref|>text<|/ref|><|det|>[[77, 259, 160, 281]]<|/det|>
又 \(CD = AB = \sqrt{6}\)  

<|ref|>text<|/ref|><|det|>[[68, 301, 463, 323]]<|/det|>
即有 \(DG^{2} + CG^{2} = CD^{2}\) ， \(DG\bot CG\) 3  

<|ref|>text<|/ref|><|det|>[[68, 331, 264, 352]]<|/det|>
又 \(CG\cap EF = G\) ， \(CG\) ， \(EF\subset\) 平面 \(BCEF\)  

<|ref|>text<|/ref|><|det|>[[68, 355, 463, 399]]<|/det|>
\(\therefore DG\bot\) 平面 \(BCEF\) 5又 \(DG\subset\) 平面 \(AFED\)  

<|ref|>text<|/ref|><|det|>[[68, 400, 463, 420]]<|/det|>
平面 \(AFED\bot\) 平面 \(BCEF\) 6  

<|ref|>text<|/ref|><|det|>[[72, 421, 166, 440]]<|/det|>
（2）连接 \(DF\) ， \(DB\)  

<|ref|>text<|/ref|><|det|>[[68, 441, 463, 465]]<|/det|>
由（1）知 \(DG\bot\) 平面 \(BCEF\) ，同理 \(CG\bot\) 平面 \(AFED\) 7  

<|ref|>text<|/ref|><|det|>[[68, 465, 463, 502]]<|/det|>
且 \(S_{\text{菱形BCEF}} = 2\times \sqrt{3} = 2\sqrt{3}\) ， \(S_{\Delta ADF} = \frac{1}{2}\times 2\times \sqrt{3} = \sqrt{3}\) 9  

<|ref|>equation<|/ref|><|det|>[[68, 508, 400, 546]]<|/det|>
\[V = V_{D - BCEF} + V_{D - ABF} = V_{D - BCEF} + V_{B - ADF} = \frac{1}{3} S_{\text{菱形BCEF}}\cdot DG + \frac{1}{3} S_{\Delta ADF}\cdot CG\]  

<|ref|>equation<|/ref|><|det|>[[68, 550, 463, 610]]<|/det|>
\[= \frac{1}{3}\times 2\sqrt{3}\times \sqrt{3} +\frac{1}{3}\times \sqrt{3}\times \sqrt{3}\quad \dots \dots \dots \dots \dots \dots \dots \dots \dots \dots \dots \dots \dots \dots \dots \dots \dots \dots \dots \dots \quad (12)\]  

<|ref|>text<|/ref|><|det|>[[68, 620, 463, 664]]<|/det|>
20. 解：（1） \(f^{\prime}(x) = \frac{-mx^{2} + 2(m - 1)x + 4}{e^{x}} = \frac{-(mx + 2)(x - 2)}{e^{x}} (m > 0)\) 1  

<|ref|>text<|/ref|><|det|>[[68, 675, 463, 710]]<|/det|>
令 \(f^{\prime}(x) = 0\) ，解得 \(x = - \frac{2}{m}\) 或 \(x = 2\) ，且 \(- \frac{2}{m} < 2\) 2  

<|ref|>text<|/ref|><|det|>[[68, 718, 357, 757]]<|/det|>
当 \(x\in (-\infty , - \frac{2}{m} ]\) 时， \(f^{\prime}(x)\leq 0\) ，当 \(x\in (- \frac{2}{m},2)\) 时， \(f^{\prime}(x) > 0\)  

<|ref|>text<|/ref|><|det|>[[68, 767, 463, 790]]<|/det|>
当 \(x\in [2, + \infty)\) 时， \(f^{\prime}(x)\leq 0\) 4  

<|ref|>text<|/ref|><|det|>[[68, 803, 463, 840]]<|/det|>
即 \(f(x)\) 的单调增区间为 \((- \frac{2}{m},2)\) ，单调减区间为 \((- \infty , - \frac{2}{m} ]\) ， \([2, + \infty)\) 5  

<|ref|>text<|/ref|><|det|>[[72, 849, 463, 872]]<|/det|>
（2）由（1）知，当 \(m > 0,x\in [1,2]\) 时， \(f^{\prime}(x) > 0\) 恒成立 6  

<|ref|>text<|/ref|><|det|>[[508, 108, 645, 130]]<|/det|>
所以 \(f(x)\) 在 \([1,2]\) 上为增函数，  

<|ref|>text<|/ref|><|det|>[[508, 142, 904, 190]]<|/det|>
即 \(f(x)_{\mathrm{max}} = f(2) = \frac{4m + 2}{e^{2}}\) ， \(f(x)_{\mathrm{min}} = f(1) = \frac{m}{e}\) 8  

<|ref|>text<|/ref|><|det|>[[508, 195, 904, 230]]<|/det|>
\(f(x_{1}) - f(x_{2})\) 的最大值为 \(g(m) = f(x)_{\mathrm{max}} - f(x)_{\mathrm{min}} = \frac{(4 - e)m + 2}{e^{2}}\) 9  

<|ref|>text<|/ref|><|det|>[[508, 234, 904, 270]]<|/det|>
\(\therefore \frac{4}{B}\geq [f(x_{1}) - f(x_{2})]\) 恒成立 10  

<|ref|>text<|/ref|><|det|>[[508, 272, 904, 308]]<|/det|>
\(\therefore \frac{4}{e^{2}}\geq \frac{(4 - e)m + 2}{e^{2}}\)  

<|ref|>text<|/ref|><|det|>[[512, 312, 904, 352]]<|/det|>
即 \(m\leq \frac{2}{4 - e}\) 11  

<|ref|>text<|/ref|><|det|>[[508, 366, 652, 405]]<|/det|>
又 \(m > 0\) \(\therefore m\in \left(0,\frac{2}{4 - e}\right]\)  

<|ref|>text<|/ref|><|det|>[[508, 432, 904, 470]]<|/det|>
故 \(m\) 的取值范围 \(\left(0,\frac{2}{4 - e}\right)\) 12  

<|ref|>text<|/ref|><|det|>[[508, 499, 904, 536]]<|/det|>
21. 解：（1） \(\because e = \frac{c}{a} = \frac{\sqrt{2}}{2}\) \(\therefore c^{2} = \frac{1}{2} a^{2}\) \(\therefore b^{2} = a^{2} - c^{2} = \frac{1}{2} a^{2}\) 2  

<|ref|>text<|/ref|><|det|>[[508, 545, 904, 604]]<|/det|>
：椭圆的中心 \(o\) 到直线 \(x + y - 2b = 0\) 的距离为 \(5\sqrt{2}\) \(\therefore \frac{| - 2b|}{\sqrt{2}} = 5\sqrt{2}\) ， \(\therefore b = 5\dots b^{2} = 25,a^{2} = 2b^{2} = 50\)  

<|ref|>text<|/ref|><|det|>[[508, 620, 904, 657]]<|/det|>
：椭圆 \(C\) 的方程为 \(\frac{x^{2}}{50} +\frac{y^{2}}{25} = 1\) 4  

<|ref|>text<|/ref|><|det|>[[512, 660, 864, 682]]<|/det|>
（2）由（1）可知 \(F(5,0)\) ，由题可知直线 \(AB\) 的方程为 \(y = \sqrt{2} (x - 5)\) ，与椭圆 \(C\)  

<|ref|>text<|/ref|><|det|>[[508, 686, 904, 770]]<|/det|>
的方程联立 \(\left\{ \begin{array}{l l}{y = \sqrt{2} (x - 5)}\\ {\frac{x^{2}}{50} +\frac{y^{2}}{25} = 1} \end{array} \right.\) ，消去 \(y\) 得 \(x^{2} - 8x + 10 = 0\) 设 \(A(x_{1},y_{1})\) ， \(B(x_{2},y_{2})\) ，则有 \(x_{1} + x_{2} = 8,x_{1}x_{2} = 10\) 6  

<|ref|>text<|/ref|><|det|>[[508, 775, 904, 796]]<|/det|>
设 \(Q(x,y)\) ，由 \(\overrightarrow{OQ} = \lambda \overrightarrow{OA} +\mu \overrightarrow{OB}\) 得 \((x,y) = \lambda (x_{1},y_{1}) + \mu (x_{2},y_{2}) = (\lambda x_{1} + \mu x_{2},\lambda y_{1} + \mu y_{2})\)  

<|ref|>text<|/ref|><|det|>[[508, 802, 904, 833]]<|/det|>
\(\therefore \left\{ \begin{array}{l l}{x = \lambda x_{1} + \mu x_{2}}\\ {y = \lambda y_{1} + \mu y_{2}} \end{array} \right.\) 7