<|ref|>image<|/ref|><|det|>[[204, 123, 805, 533]]<|/det|>  

<|ref|>sub_title<|/ref|><|det|>[[188, 550, 338, 567]]<|/det|>
## 1. 三角恒等变换  

<|ref|>text<|/ref|><|det|>[[183, 577, 782, 644]]<|/det|>
万能置换公式： \(\sin x = \frac{2\tan\frac{x}{2}}{1 + \tan^{2}\frac{x}{2}};\cos x = \frac{1 - \tan^{2}\frac{x}{2}}{1 + \tan^{2}\frac{x}{2}};\tan x = \frac{2\tan\frac{x}{2}}{1 - \tan^{2}\frac{x}{2}};\)  

<|ref|>text<|/ref|><|det|>[[191, 653, 338, 669]]<|/det|>
（1）积化和差公式  

<|ref|>text<|/ref|><|det|>[[185, 678, 857, 760]]<|/det|>
\(\sin A\cos B = \frac{1}{2} [\sin (A + B) + \sin (A - B)];\cos A\sin B = \frac{1}{2} [\sin (A + B) - \sin (A - B)];\) \(\cos A\cos B = \frac{1}{2} [\cos (A + B) + \cos (A - B)];\sin A\sin B = \frac{1}{2} [\cos (A - B) - \cos (A + B)];\)  

<|ref|>text<|/ref|><|det|>[[192, 772, 340, 788]]<|/det|>
（2）和差化积公式  

<|ref|>equation<|/ref|><|det|>[[185, 799, 816, 877]]<|/det|>
\[\sin A + \sin B = 2\sin \frac{A + B}{2}\cos \frac{A - B}{2};\sin A - \sin B = 2\cos \frac{A + B}{2}\sin \frac{A - B}{2};\] \[\cos A + \cos B = 2\cos \frac{A + B}{2}\cos \frac{A - B}{2};\cos A - \cos B = -2\sin \frac{A + B}{2}\sin \frac{A - B}{2};\]